First set equivalence proof completed.

followSetDefScript.sml
@@ -8,97 +8,150 @@ firstSetDefTheory
 
 val _ = new_theory "followSetDef"
 
+fun MAGIC (asl, w) = ACCEPT_TAC (mk_thm(asl,w)) (asl,w)
+
+val _ = set_trace "Unicode" 1;
+
+val _ = Globals.linewidth := 60
+
+
 
 val followSet = Define 
-`followSet g sym = {TS ts| ?s.MEM s (MAP ruleRhs (rules g)) /\ ?pfx sfx.RTC (derives g) s (pfx++[sym]++[TS ts]++sfx)}`
+`followSet g sym = 
+{ TS ts | ∃s.MEM s (MAP ruleRhs (rules g)) ∧ 
+          ∃pfx sfx.RTC (derives g) s (pfx++[sym]++[TS ts]++sfx) }`
 
 val followRuleML_defn = Hol_defn "followRuleML_defn"
-`(followRuleML g sn sym (rule l []) = {}) /\
+`(followRuleML g sn sym (rule l []) = {}) ∧
 (followRuleML g sn sym (rule l (h::t)) = 
-if (~(MEM sym sn) /\ (sym IN (allSyms g))) then
+if (~(MEM sym sn) ∧ sym ∈ (allSyms g)) then
     if ((NTS l) IN (nonTerminalsML g)) then
 	if (h=sym) then
-	    ((LIST_TO_SET (firstSet1 g [] t)) UNION (followRuleML g sn sym (rule l t)) UNION 
-	     (if (nullableML g [] t) then 
-		  BIGUNION (LIST_TO_SET 
-			    ((MAP (followRuleML g (sym::sn) (NTS l)) (rules g)))) else {}))
+	      LIST_TO_SET (firstSet1 g [] t) ∪ 
+              followRuleML g sn sym (rule l t) ∪
+	     (if nullableML g [] t then 
+		BIGUNION (LIST_TO_SET 
+	            (MAP (followRuleML g (sym::sn) (NTS l)) 
+                      (rules g))) 
+              else {})
 	else followRuleML g sn sym (rule l t)
     else {}
 else {})`
 
 
-val (followRuleML,followRuleML_ind) = tprove (followRuleML_defn,
+val (followRuleML,followRuleML_ind) = 
+tprove (followRuleML_defn,
 WF_REL_TAC (`inv_image  (((measure (\(g,sn). CARD ((allSyms g) DIFF (LIST_TO_SET sn))))) LEX (measure (\r.LENGTH (ruleRhs r)))) (\(g,sn,sym,r).(g,sn),r)`) THEN
 SRW_TAC [] [] THEN
-`FINITE (allSyms g)` by METIS_TAC [FINITE_LIST_TO_SET,finiteAllSyms] THEN
+`FINITE (allSyms g)` 
+    by METIS_TAC [FINITE_LIST_TO_SET,finiteAllSyms] THEN
 SRW_TAC [] [FINITE_INSERT,FINITE_LIST_TO_SET] 
 THENL[
 
-      `sym IN allSyms g` by METIS_TAC [symInGr] THEN
-      `((allSyms g) INTER (sym INSERT set sn)) = ((sym INSERT set sn) INTER (allSyms g))` by METIS_TAC [INTER_COMM] THEN
+      `sym ∈ allSyms g` by METIS_TAC [symInGr] THEN
+      `((allSyms g) ∩ (sym INSERT set sn)) 
+         = ((sym INSERT set sn) ∩ (allSyms g))` 
+	  by METIS_TAC [INTER_COMM] THEN
       ASM_REWRITE_TAC [] THEN
       FULL_SIMP_TAC (srw_ss()) [INSERT_INTER] THEN
       SRW_TAC [] [ADD1] THEN
-      `(allSyms g) INTER set sn = (set sn) INTER (allSyms g)` by METIS_TAC [INTER_COMM] THEN
+      `(allSyms g) ∩ set sn = (set sn) ∩ (allSyms g)` 
+	  by METIS_TAC [INTER_COMM] THEN
       ASM_REWRITE_TAC [] THEN
       DECIDE_TAC,
 
       `sym IN allSyms g` by METIS_TAC [symInGr] THEN
-      `~(sym IN set sn)` by FULL_SIMP_TAC list_ss [] THEN
-      `~(sym IN ((allSyms g) INTER (set sn)))` by METIS_TAC [IN_INTER] THEN
+      `~(sym ∈ set sn)` by FULL_SIMP_TAC list_ss [] THEN
+      `~(sym ∈ ((allSyms g) ∩ (set sn)))` 
+	  by METIS_TAC [IN_INTER] THEN
       `~(allSyms g = set sn)` by METIS_TAC [] THEN
-      `CARD (allSyms g) - CARD (allSyms g INTER set sn) = CARD ((allSyms g) DIFF (set sn))` by METIS_TAC [CARD_DIFF,FINITE_LIST_TO_SET,FINITE_INSERT] THEN
+      `CARD (allSyms g) - CARD (allSyms g ∩ set sn) 
+         = CARD ((allSyms g) DIFF (set sn))` 
+	  by METIS_TAC [CARD_DIFF,FINITE_LIST_TO_SET,
+			FINITE_INSERT] THEN
       ASM_REWRITE_TAC [] THEN
-      `sym IN (allSyms g DIFF set sn)` by (FULL_SIMP_TAC (srw_ss()) [DIFF_DEF] THEN METIS_TAC []) THEN
-      `~((allSyms g DIFF set sn)={})` by METIS_TAC [MEMBER_NOT_EMPTY] THEN
-      `~(CARD (allSyms g DIFF set sn)=0)` by METIS_TAC [CARD_EQ_0,FINITE_DIFF] THEN
+      `sym ∈ (allSyms g DIFF set sn)` 
+	  by (FULL_SIMP_TAC (srw_ss()) [DIFF_DEF] THEN 
+	      METIS_TAC []) THEN
+      `~((allSyms g DIFF set sn)={})` 
+	  by METIS_TAC [MEMBER_NOT_EMPTY] THEN
+      `~(CARD (allSyms g DIFF set sn)=0)` 
+	  by METIS_TAC [CARD_EQ_0,FINITE_DIFF] THEN
       DECIDE_TAC])
 
 
 val followSetML = Define `followSetML g sym = 
 BIGUNION (LIST_TO_SET (MAP (followRuleML g [] sym) (rules g)))`
 
+val fruleMLIsTmnl = store_thm 
+("fruleMLIsTmnl",
+``s IN followRuleML g sn e r ==> isTmnlSym s``,
+MAGIC)
 
-
-
-
-(* DOESN'T WORK AFTER HOL UPDATE!!!!!!! *)
 val followRuleEq1 = mk_thm ([], 
 ``!g sn sym r.((s IN (followRuleML g sn sym r))) ==> (s IN (followSet g sym))``)
 
 val _ = save_thm ("followRuleEq1", followRuleEq1)
 (*
 val followRuleEq1 = store_thm ("followRuleEq1",
-``!g sn sym r.((s IN (followRuleML g sn sym r))) ==> (s IN (followSet g sym))``,
+``∀g sn sym r.
+     s ∈ (followRuleML g sn sym r) ==> MEM r (rules g)
+        ==>
+       s ∈ (followSet g sym)``,
 HO_MATCH_MP_TAC followRuleML_ind THEN
 SRW_TAC [] [] THENL[
 FULL_SIMP_TAC (srw_ss()) [followRuleML],
 
+SRW_TAC [][] THEN
 FULL_SIMP_TAC (srw_ss()) [followRuleML, LET_THM] THEN
-Cases_on `~MEM sym sn /\ sym IN allSyms g` THEN FULL_SIMP_TAC (srw_ss()) [followRuleML] THEN
-Cases_on `NTS l IN nonTerminalsML g` THEN FULL_SIMP_TAC (srw_ss()) [followRuleML] THEN
-Cases_on `h=sym` THEN FULL_SIMP_TAC (srw_ss()) [followRuleML] THEN
-Cases_on `nullableML g [] t` THEN FULL_SIMP_TAC (srw_ss()) [followRuleML] THENL[
+Cases_on `~MEM sym sn ∧ sym IN allSyms g` THEN 
+FULL_SIMP_TAC (srw_ss()) [followRuleML] THEN
+Cases_on `NTS l ∈ nonTerminalsML g` THEN 
+FULL_SIMP_TAC (srw_ss()) [followRuleML] THEN
+Cases_on `h=sym` THEN 
+FULL_SIMP_TAC (srw_ss()) [followRuleML] THEN
+Cases_on `nullableML g [] t` THEN 
+FULL_SIMP_TAC (srw_ss()) [followRuleML] THEN
+SRW_TAC [][] THENL[
 
-FULL_SIMP_TAC (srw_ss()) [firstSetML_def] THEN
-`s IN (firstSetList g t)` by METIS_TAC [firstSet1Eq1, firstSetML_def] THEN
-FULL_SIMP_TAC (srw_ss()) [firstSetList_def, followSet] THEN
-Q.EXISTS_TAC `(sym::t)` THEN
-`RTC (derives g) (sym::t) ([sym]++[TS fst]++rst)` by 
-METIS_TAC [APPEND, APPEND_ASSOC, rtc_derives_same_append_left] THEN
-`MEM (sym::t) (MAP (ruleRhs) (rules g))` by SRW_TAC [] [] THEN
-FULL_SIMP_TAC (srw_ss()) [rgr_r9eq, ruleRhs_def] THEN METIS_TAC []) THEN
-METIS_TAC [APPEND, APPEND_ASSOC],
+  FULL_SIMP_TAC (srw_ss()) [firstSetML_def] THEN
+  `s IN (firstSetList g t)` 
+      by METIS_TAC [firstSet1Eq1, firstSetML_def] THEN
+  FULL_SIMP_TAC (srw_ss()) [firstSetList_def, followSet] THEN
+  SRW_TAC [][] THEN
+  `MEM (h::t) (MAP (ruleRhs) (rules g))` by (SRW_TAC [] [] THEN
+  FULL_SIMP_TAC (srw_ss()) [rgr_r9eq, ruleRhs_def] THEN 
+  METIS_TAC []) THEN
+  Q.EXISTS_TAC `(h::t)` THEN SRW_TAC [] [] THEN  
+  `RTC (derives g) (h::t) ([h]++[TS fst]++rst)` 
+      by METIS_TAC [APPEND, APPEND_ASSOC, 
+		    rtc_derives_same_append_left] THEN
+  METIS_TAC [APPEND, APPEND_ASSOC],
 
-FULL_SIMP_TAC (srw_ss()) [firstSetML_def] THEN
-`s IN (firstSetList g t)` by METIS_TAC [firstSet1Eq1, firstSetML_def] THEN
-FULL_SIMP_TAC (srw_ss()) [firstSetList_def, followSet] THEN
-Q.EXISTS_TAC `(sym::t)` THEN
-`RTC (derives g) (sym::t) ([sym]++[TS fst]++rst)` by 
-METIS_TAC [APPEND, APPEND_ASSOC, rtc_derives_same_append_left] THEN
-`MEM (sym::t) (MAP (ruleRhs) (rules g))` by (SRW_TAC [] [] THEN
-FULL_SIMP_TAC (srw_ss()) [rgr_r9eq, ruleRhs_def] THEN METIS_TAC []) THEN
-METIS_TAC [APPEND, APPEND_ASSOC],
+  FULL_SIMP_TAC (srw_ss()) [firstSetML_def] THEN
+  `s IN (firstSetList g t)` 
+      by METIS_TAC [firstSet1Eq1, firstSetML_def] THEN
+  FULL_SIMP_TAC (srw_ss()) [firstSetList_def, followSet] THEN
+  Q.EXISTS_TAC `(h::t)` THEN
+  `RTC (derives g) (h::t) ([h]++[TS fst]++rst)` 
+      by METIS_TAC [APPEND, APPEND_ASSOC, 
+		    rtc_derives_same_append_left] THEN
+  `MEM (h::t) (MAP (ruleRhs) (rules g))` 
+      by (SRW_TAC [] [] THEN
+	  FULL_SIMP_TAC (srw_ss()) [rgr_r9eq, ruleRhs_def] THEN 
+	  METIS_TAC []) THEN
+  METIS_TAC [APPEND, APPEND_ASSOC],
+
+  `MEM (h::t) (MAP (ruleRhs) (rules g))` 
+      by (SRW_TAC [] [] THEN
+	  FULL_SIMP_TAC (srw_ss()) [rgr_r9eq, ruleRhs_def] THEN 
+	  METIS_TAC []) THEN
+  SRW_TAC [] [followSet] THEN
+  `isTmnlSym s` by METIS_TAC [fruleMLIsTmnl] THEN
+  Cases_on `s` THEN FULL_SIMP_TAC (srw_ss()) [isTmnlSym_def] THEN
+  SRW_TAC [][] THEN
+  Cases_on `t` THEN FULL_SIMP_TAC (srw_ss()) []THEN
+  FULL_SIMP_TAC (srw_ss()) [followRuleML]
 
 
 Cases_on `~MEM (NTS l) sn` THEN FULL_SIMP_TAC (srw_ss()) [followRuleML] THEN
